src/dafny/Thread.dfy
@@ -1,0 +1,28 @@
+include "Endo.dfy"
+
+class Thread {
+    var tid:int;
+    var pc:int;
+    var sp:int;
+    var instructions:seq<string>;
+    var endokernel:Endokernel;
+
+    constructor (tid:int, pc:int, sp:int, instructions:seq<string>, endokernel:Endokernel)
+    ensures this.endokernel == old(endokernel)
+     {
+        this.tid := tid;
+        this.pc := pc;
+        this.sp := sp;
+        this.instructions := instructions;
+        this.endokernel := endokernel;
+    }
+
+    method exec() modifies this, endokernel {
+        if (0 <= pc < |instructions|) {
+            print "Executing instruction " + instructions[pc] + " in Process\n";
+            this.endokernel.trap(instructions[pc]);
+            pc := pc + 1;
+        }
+    }
+
+}
